{-# OPTIONS --without-K --exact-split #-}

module 03-inductive-types where

import 02-natural-numbers
open 02-natural-numbers public


-- The unit type

data unit : UU lzero where
  star : unit
  
ğŸ™ = unit

ind-unit : {i : Level} {P : unit â†’ UU i} â†’ P star â†’ ((x : unit) â†’ P x)
ind-unit p star = p

-- The empty type

data empty : UU lzero where

ğŸ˜ = empty

ind-empty : {i : Level} {P : empty â†’ UU i} â†’ ((x : empty) â†’ P x)
ind-empty ()

Â¬ : {i : Level} â†’ UU i â†’ UU i
Â¬ A = A â†’ empty

-- The type of booleans

data bool : UU lzero where
  true false : bool

neg-ğŸš : bool â†’ bool
neg-ğŸš true = false
neg-ğŸš false = true

conjunction-ğŸš : bool â†’ (bool â†’ bool)
conjunction-ğŸš true true = true
conjunction-ğŸš true false = false
conjunction-ğŸš false true = false
conjunction-ğŸš false false = false

disjunction-ğŸš : bool â†’ (bool â†’ bool)
disjunction-ğŸš true true = true
disjunction-ğŸš true false = true
disjunction-ğŸš false true = true
disjunction-ğŸš false false = false

-- Coproducts

data coprod {i j : Level} (A : UU i) (B : UU j) : UU (i âŠ” j)  where
  inl : A â†’ coprod A B
  inr : B â†’ coprod A B

ind-coprod : {i j k : Level} {A : UU i} {B : UU j} (C : coprod A B â†’ UU k) â†’
  ((x : A) â†’ C (inl x)) â†’ ((y : B) â†’ C (inr y)) â†’
  (t : coprod A B) â†’ C t
ind-coprod C f g (inl x) = f x
ind-coprod C f g (inr x) = g x

-- Dependent pair types

data Î£ {i j : Level} (A : UU i) (B : A â†’ UU j) : UU (i âŠ” j) where
  pair : (x : A) â†’ (B x â†’ Î£ A B)

ind-Î£ : {i j k : Level} {A : UU i} {B : A â†’ UU j} {C : Î£ A B â†’ UU k} â†’
  ((x : A) (y : B x) â†’ C (pair x y)) â†’ ((t : Î£ A B) â†’ C t)
ind-Î£ f (pair x y) = f x y

pr1 : {i j : Level} {A : UU i} {B : A â†’ UU j} â†’ Î£ A B â†’ A
pr1 (pair a b) = a

pr2 : {i j : Level} {A : UU i} {B : A â†’ UU j} â†’ (t : Î£ A B) â†’ B (pr1 t)
pr2 (pair a b) = b

-- Cartesian products

prod : {i j : Level} (A : UU i) (B : UU j) â†’ UU (i âŠ” j)
prod A B = Î£ A (Î» a â†’ B)

pair' :
  {i j : Level} {A : UU i} {B : UU j} â†’ A â†’ B â†’ prod A B
pair' = pair

_Ã—_ :  {i j : Level} (A : UU i) (B : UU j) â†’ UU (i âŠ” j)
A Ã— B = prod A B

-- The type of integers

â„¤ : UU lzero
â„¤ = coprod â„• (coprod unit â„•)

-- Inclusion of the negative integers

in-neg : â„• â†’ â„¤
in-neg n = inl n

-- Negative one

neg-one-â„¤ : â„¤
neg-one-â„¤ = in-neg zero-â„•

-- Zero

zero-â„¤ : â„¤
zero-â„¤ = inr (inl star)

-- One

one-â„¤ : â„¤
one-â„¤ = inr (inr zero-â„•)

-- Inclusion of the positive integers

in-pos : â„• â†’ â„¤
in-pos n = inr (inr n)

{- We prove an induction principle for the integers. -}

ind-â„¤ : {i : Level} (P : â„¤ â†’ UU i) â†’ P neg-one-â„¤ â†’ ((n : â„•) â†’ P (inl n) â†’ P (inl (succ-â„• n))) â†’ P zero-â„¤ â†’ P one-â„¤ â†’ ((n : â„•) â†’ P (inr (inr (n))) â†’ P (inr (inr (succ-â„• n)))) â†’ (k : â„¤) â†’ P k
ind-â„¤ P p-1 p-S p0 p1 pS (inl zero-â„•) = p-1
ind-â„¤ P p-1 p-S p0 p1 pS (inl (succ-â„• x)) = p-S x (ind-â„¤ P p-1 p-S p0 p1 pS (inl x))
ind-â„¤ P p-1 p-S p0 p1 pS (inr (inl star)) = p0
ind-â„¤ P p-1 p-S p0 p1 pS (inr (inr zero-â„•)) = p1
ind-â„¤ P p-1 p-S p0 p1 pS (inr (inr (succ-â„• x))) = pS x (ind-â„¤ P p-1 p-S p0 p1 pS (inr (inr (x))))

succ-â„¤ : â„¤ â†’ â„¤
succ-â„¤ (inl zero-â„•) = zero-â„¤
succ-â„¤ (inl (succ-â„• x)) = inl x
succ-â„¤ (inr (inl star)) = one-â„¤
succ-â„¤ (inr (inr x)) = inr (inr (succ-â„• x))

-- Exercise 3.9
-- In this exercise we were asked to show that 1 + 1 satisfies the induction principle of the booleans. In other words, type theory cannot distinguish the booleans from the type 1 + 1. We will see later that they are indeed equivalent types.
t0 : coprod unit unit
t0 = inl star

t1 : coprod unit unit
t1 = inr star

ind-coprod-unit-unit : {i : Level} {P : coprod unit unit â†’ UU i} â†’
  P t0 â†’ P t1 â†’ (x : coprod unit unit) â†’ P x
ind-coprod-unit-unit p0 p1 (inl star) = p0
ind-coprod-unit-unit p0 p1 (inr star) = p1

-- Exercise 3.11
pred-â„¤ : â„¤ â†’ â„¤
pred-â„¤ (inl x) = inl (succ-â„• x)
pred-â„¤ (inr (inl star)) = inl zero-â„•
pred-â„¤ (inr (inr zero-â„•)) = inr (inl star)
pred-â„¤ (inr (inr (succ-â„• x))) = inr (inr x)

-- Exercise 3.12
add-â„¤ : â„¤ â†’ â„¤ â†’ â„¤
add-â„¤ (inl zero-â„•) l = pred-â„¤ l
add-â„¤ (inl (succ-â„• x)) l = pred-â„¤ (add-â„¤ (inl x) l)
add-â„¤ (inr (inl star)) l = l
add-â„¤ (inr (inr zero-â„•)) l = succ-â„¤ l
add-â„¤ (inr (inr (succ-â„• x))) l = succ-â„¤ (add-â„¤ (inr (inr x)) l)

neg-â„¤ : â„¤ â†’ â„¤
neg-â„¤ (inl x) = inr (inr x)
neg-â„¤ (inr (inl star)) = inr (inl star)
neg-â„¤ (inr (inr x)) = inl x

-- Multiplication on â„¤

mul-â„¤ : â„¤ â†’ â„¤ â†’ â„¤
mul-â„¤ (inl zero-â„•) l = neg-â„¤ l
mul-â„¤ (inl (succ-â„• x)) l = add-â„¤ (neg-â„¤ l) (mul-â„¤ (inl x) l)
mul-â„¤ (inr (inl star)) l = zero-â„¤
mul-â„¤ (inr (inr zero-â„•)) l = l
mul-â„¤ (inr (inr (succ-â„• x))) l = add-â„¤ l (mul-â„¤ (inr (inr x)) l)

-- Extend the Fibonacci sequence to â„¤ in the obvious way
Fibonacci-â„¤ : â„¤ â†’ â„¤
Fibonacci-â„¤ (inl zero-â„•) = one-â„¤
Fibonacci-â„¤ (inl (succ-â„• zero-â„•)) = neg-one-â„¤
Fibonacci-â„¤ (inl (succ-â„• (succ-â„• x))) =
  add-â„¤ (Fibonacci-â„¤ (inl x)) (neg-â„¤ (Fibonacci-â„¤ (inl (succ-â„• x))))
Fibonacci-â„¤ (inr (inl star)) = zero-â„¤
Fibonacci-â„¤ (inr (inr zero-â„•)) = one-â„¤
Fibonacci-â„¤ (inr (inr (succ-â„• zero-â„•))) = one-â„¤
Fibonacci-â„¤ (inr (inr (succ-â„• (succ-â„• x)))) =
  add-â„¤ (Fibonacci-â„¤ (inr (inr x))) (Fibonacci-â„¤ (inr (inr (succ-â„• x))))

-- Exercise

exclusive-disjunction-ğŸš : bool â†’ (bool â†’ bool)
exclusive-disjunction-ğŸš true true = false
exclusive-disjunction-ğŸš true false = true
exclusive-disjunction-ğŸš false true = true
exclusive-disjunction-ğŸš false false = false

implication-ğŸš : bool â†’ (bool â†’ bool)
implication-ğŸš true true = true
implication-ğŸš true false = false
implication-ğŸš false true = true
implication-ğŸš false false = true

bi-implication-ğŸš : bool â†’ (bool â†’ bool)
bi-implication-ğŸš true true = true
bi-implication-ğŸš true false = false
bi-implication-ğŸš false true = false
bi-implication-ğŸš false false = true

peirce-arrow-ğŸš : bool â†’ (bool â†’ bool)
peirce-arrow-ğŸš true true = false
peirce-arrow-ğŸš true false = false
peirce-arrow-ğŸš false true = false
peirce-arrow-ğŸš false false = true

sheffer-stroke-ğŸš : bool â†’ (bool â†’ bool)
sheffer-stroke-ğŸš true true = false
sheffer-stroke-ğŸš true false = true
sheffer-stroke-ğŸš false true = true
sheffer-stroke-ğŸš false false = true

