{-# OPTIONS --without-K --exact-split #-}

module 10-number-theory where

import 09-truncation-levels
open 09-truncation-levels public

-- Section 10.1 Decidability.

{- Recall that a proposition P is decidable if P + (Â¬ P) holds. -}

classical-Prop :
  (l : Level) â†’ UU (lsuc l)
classical-Prop l = Î£ (hProp l) (Î» P â†’ decide (pr1 P))

abstract
  is-decidable-Eq-â„• :
    (m n : â„•) â†’ decide (Eq-â„• m n)
  is-decidable-Eq-â„• zero-â„• zero-â„• = inl star
  is-decidable-Eq-â„• zero-â„• (succ-â„• n) = inr id
  is-decidable-Eq-â„• (succ-â„• m) zero-â„• = inr id
  is-decidable-Eq-â„• (succ-â„• m) (succ-â„• n) = is-decidable-Eq-â„• m n

abstract
  is-decidable-leq-â„• :
    (m n : â„•) â†’ decide (leq-â„• m n)
  is-decidable-leq-â„• zero-â„• zero-â„• = inl star
  is-decidable-leq-â„• zero-â„• (succ-â„• n) = inl star
  is-decidable-leq-â„• (succ-â„• m) zero-â„• = inr id
  is-decidable-leq-â„• (succ-â„• m) (succ-â„• n) = is-decidable-leq-â„• m n

abstract
  is-decidable-le-â„• :
    (m n : â„•) â†’ decide (le-â„• m n)
  is-decidable-le-â„• zero-â„• zero-â„• = inr id
  is-decidable-le-â„• zero-â„• (succ-â„• n) = inl star
  is-decidable-le-â„• (succ-â„• m) zero-â„• = inr id
  is-decidable-le-â„• (succ-â„• m) (succ-â„• n) = is-decidable-le-â„• m n

{- We say that a type has decidable equality if we can decide whether x = y
   holds for any x,y:A. -}
   
has-decidable-equality : {l : Level} (A : UU l) â†’ UU l
has-decidable-equality A = (x y : A) â†’ decide (Id x y)

{- Next, we show that types with decidable equality are sets. To see this, we 
   will construct a fiberwise equivalence with the binary relation R that is
   defined by R x y := unit if (x = y), and empty otherwise. In order to define
   this relation, we first define a type family over ((x = y) + Â¬(x = y)) that 
   returns unit on the left and empty on the right. -}
   
splitting-decidable-equality : {l : Level} (A : UU l) (x y : A) â†’
  decide (Id x y) â†’ UU lzero
splitting-decidable-equality A x y (inl p) = unit
splitting-decidable-equality A x y (inr f) = empty

abstract
  is-prop-splitting-decidable-equality : {l : Level} (A : UU l) (x y : A) â†’
    (t : decide (Id x y)) â†’
    is-prop (splitting-decidable-equality A x y t)
  is-prop-splitting-decidable-equality A x y (inl p) = is-prop-unit
  is-prop-splitting-decidable-equality A x y (inr f) = is-prop-empty

reflexive-splitting-decidable-equality : {l : Level} (A : UU l) (x : A) â†’
  (t : decide (Id x x)) â†’ splitting-decidable-equality A x x t
reflexive-splitting-decidable-equality A x (inl p) = star
reflexive-splitting-decidable-equality A x (inr f) =
  ind-empty {P = Î» t â†’ splitting-decidable-equality A x x (inr f)} (f refl)

eq-splitting-decidable-equality : {l : Level} (A : UU l) (x y : A) â†’
  (t : decide (Id x y)) â†’
  splitting-decidable-equality A x y t â†’ Id x y
eq-splitting-decidable-equality A x y (inl p) t = p
eq-splitting-decidable-equality A x y (inr f) t =
  ind-empty {P = Î» s â†’ Id x y} t 

abstract
  is-set-has-decidable-equality : {l : Level} (A : UU l) â†’
    has-decidable-equality A â†’ is-set A
  is-set-has-decidable-equality A d =
    is-set-prop-in-id
      ( Î» x y â†’ splitting-decidable-equality A x y (d x y))
      ( Î» x y â†’ is-prop-splitting-decidable-equality A x y (d x y))
      ( Î» x â†’ reflexive-splitting-decidable-equality A x (d x x))
      ( Î» x y â†’ eq-splitting-decidable-equality A x y (d x y))

abstract
  has-decidable-equality-coprod : {l1 l2 : Level} {A : UU l1} {B : UU l2} â†’
    has-decidable-equality A â†’ has-decidable-equality B â†’
    has-decidable-equality (coprod A B)
  has-decidable-equality-coprod dec-A dec-B (inl x) (inl y) =
    functor-coprod
      ( ap inl)
      ( Î» f p â†’ f (inv-is-equiv (is-emb-inl _ _ x y) p))
      ( dec-A x y)
  has-decidable-equality-coprod {A = A} {B = B} dec-A dec-B (inl x) (inr y) =
    inr
      ( Î» p â†’
        inv-is-equiv
          ( is-equiv-map-raise _ empty)
          ( Eq-coprod-eq A B (inl x) (inr y) p))
  has-decidable-equality-coprod {A = A} {B = B} dec-A dec-B (inr x) (inl y) =
    inr
      ( Î» p â†’
        inv-is-equiv
          ( is-equiv-map-raise _ empty)
          ( Eq-coprod-eq A B (inr x) (inl y) p))
  has-decidable-equality-coprod dec-A dec-B (inr x) (inr y) =
    functor-coprod
      ( ap inr)
      ( Î» f p â†’ f (inv-is-equiv (is-emb-inr _ _ x y) p))
      ( dec-B x y)

{- Decidable equality of Fin n. -}

has-decidable-equality-empty :
  has-decidable-equality empty
has-decidable-equality-empty ()

has-decidable-equality-unit :
  has-decidable-equality unit
has-decidable-equality-unit star star = inl refl

abstract
  has-decidable-equality-Fin :
    (n : â„•) â†’ has-decidable-equality (Fin n)
  has-decidable-equality-Fin zero-â„• = has-decidable-equality-empty
  has-decidable-equality-Fin (succ-â„• n) =
    has-decidable-equality-coprod
      ( has-decidable-equality-Fin n)
      ( has-decidable-equality-unit)

abstract
  is-set-Fin :
    (n : â„•) â†’ is-set (Fin n)
  is-set-Fin n =
    is-set-has-decidable-equality
      ( Fin n)
      ( has-decidable-equality-Fin n)

{- Decidable equality of â„•. -}

Eq-â„•-eq : (x y : â„•) â†’ Id x y â†’ Eq-â„• x y
Eq-â„•-eq x .x refl = refl-Eq-â„• x

abstract
  is-injective-succ-â„• : (x y : â„•) â†’ Id (succ-â„• x) (succ-â„• y) â†’ Id x y
  is-injective-succ-â„• zero-â„• zero-â„• p = refl
  is-injective-succ-â„• zero-â„• (succ-â„• y) p =
    ind-empty
      { P = Î» t â†’ Id zero-â„• (succ-â„• y)}
      ( Eq-â„•-eq one-â„• (succ-â„• (succ-â„• y)) p)
  is-injective-succ-â„• (succ-â„• x) zero-â„• p =
    ind-empty
      { P = Î» t â†’ Id (succ-â„• x) zero-â„•}
      ( Eq-â„•-eq (succ-â„• (succ-â„• x)) one-â„• p)
  is-injective-succ-â„• (succ-â„• x) (succ-â„• y) p =
    ap succ-â„• (eq-Eq-â„• x y (Eq-â„•-eq (succ-â„• (succ-â„• x)) (succ-â„• (succ-â„• y)) p))

abstract
  has-decidable-equality-â„• : has-decidable-equality â„•
  has-decidable-equality-â„• zero-â„• zero-â„• = inl refl
  has-decidable-equality-â„• zero-â„• (succ-â„• y) = inr (Eq-â„•-eq zero-â„• (succ-â„• y))
  has-decidable-equality-â„• (succ-â„• x) zero-â„• = inr (Eq-â„•-eq (succ-â„• x) zero-â„•)
  has-decidable-equality-â„• (succ-â„• x) (succ-â„• y) =
    functor-coprod
      ( ap succ-â„•)
      ( Î» (f : Â¬ (Id x y)) p â†’ f (is-injective-succ-â„• x y p))
      ( has-decidable-equality-â„• x y)

{- The well-ordering principle. -}

is-minimal-element-â„• :
  {l : Level} (P : â„• â†’ UU l) (n : â„•) (p : P n) â†’ UU l
is-minimal-element-â„• P n p =
  (m : â„•) â†’ P m â†’ (leq-â„• n m)

minimal-element-â„• :
  {l : Level} (P : â„• â†’ UU l) â†’ UU l
minimal-element-â„• P = Î£ â„• (Î» n â†’ Î£ (P n) (is-minimal-element-â„• P n))

leq-zero-â„• :
  (n : â„•) â†’ leq-â„• zero-â„• n
leq-zero-â„• zero-â„• = star
leq-zero-â„• (succ-â„• n) = star

is-minimal-element-succ-â„• :
  {l : Level} (P : â„• â†’ UU l) (d : (n : â„•) â†’ decide (P n))
  (m : â„•) (pm : P (succ-â„• m))
  (is-min-m : is-minimal-element-â„• (Î» x â†’ P (succ-â„• x)) m pm) â†’
  Â¬ (P zero-â„•) â†’ is-minimal-element-â„• P (succ-â„• m) pm
is-minimal-element-succ-â„• P d m pm is-min-m neg-p0 zero-â„• p0 =
  ind-empty (neg-p0 p0)
is-minimal-element-succ-â„• P d zero-â„• pm is-min-m neg-p0 (succ-â„• n) psuccn =
  leq-zero-â„• n
is-minimal-element-succ-â„• P d (succ-â„• m) pm is-min-m neg-p0 (succ-â„• n) psuccn =
  is-minimal-element-succ-â„• (Î» x â†’ P (succ-â„• x)) (Î» x â†’ d (succ-â„• x)) m pm
    ( Î» m â†’ is-min-m (succ-â„• m))
    ( is-min-m zero-â„•)
    ( n)
    ( psuccn)
  
well-ordering-principle-succ-â„• :
  {l : Level} (P : â„• â†’ UU l) (d : (n : â„•) â†’ decide (P n))
  (n : â„•) (p : P (succ-â„• n)) â†’
  decide (P zero-â„•) â†’
  minimal-element-â„• (Î» m â†’ P (succ-â„• m)) â†’ minimal-element-â„• P
well-ordering-principle-succ-â„• P d n p (inl p0) _ =
  pair zero-â„• (pair p0 (Î» m q â†’ leq-zero-â„• m))
well-ordering-principle-succ-â„• P d n p
  (inr neg-p0) (pair m (pair pm is-min-m)) =
  pair
    ( succ-â„• m)
    ( pair pm
      ( is-minimal-element-succ-â„• P d m pm is-min-m neg-p0))

well-ordering-principle-â„• :
  {l : Level} (P : â„• â†’ UU l) (d : (n : â„•) â†’ decide (P n)) â†’
  Î£ â„• P â†’ minimal-element-â„• P
well-ordering-principle-â„• P d (pair zero-â„• p) =
  pair zero-â„• (pair p (Î» m q â†’ leq-zero-â„• m))
well-ordering-principle-â„• P d (pair (succ-â„• n) p) =
  well-ordering-principle-succ-â„• P d n p (d zero-â„•)
    ( well-ordering-principle-â„•
      ( Î» m â†’ P (succ-â„• m))
      ( Î» m â†’ d (succ-â„• m))
      ( pair n p))

{- The Pigeon hole principle. -}

{- First we write a function that counts the number of elements in a decidable
   subset of a finite set. -}

count-Fin-succ-â„• :
  {l : Level} (n : â„•) (P : Fin (succ-â„• n) â†’ classical-Prop l) â†’
  â„• â†’ decide (pr1 (pr1 (P (inr star)))) â†’ â„•
count-Fin-succ-â„• n P m (inl x) = succ-â„• m
count-Fin-succ-â„• n P m (inr x) = m

count-Fin :
  (l : Level) (n : â„•) (P : Fin n â†’ classical-Prop l) â†’ â„•
count-Fin l zero-â„• P = zero-â„•
count-Fin l (succ-â„• n) P =
  count-Fin-succ-â„• n P
    ( count-Fin l n (P âˆ˜ inl))
    ( pr2 (P (inr star)))

{- Next we prove the pigeonhole principle. -}

decidable-Eq-Fin :
  (n : â„•) (i j : Fin n) â†’ classical-Prop lzero
decidable-Eq-Fin n i j =
  pair
    ( pair (Id i j) (is-set-Fin n i j))
    ( has-decidable-equality-Fin n i j)

{-
pigeonhole-principle :
  (m n : â„•) (f : Fin n â†’ Fin m) (H : le-â„• m n) â†’
  Î£ ( Fin m) (Î» i â†’
    le-â„• one-â„•
      ( count-Fin lzero n
        ( Î» j â†’ decidable-Eq-Fin m (f j) i)))
pigeonhole-principle zero-â„• (succ-â„• n) f H = {!!}
pigeonhole-principle (succ-â„• m) n f H = {!!}
-}

-- The greatest common divisor

{- First we show that mul-â„• n is an embedding whenever n > 0. In order to do
   this, we have to show that add-â„• n is injective. -}
   
is-injective-add-â„• :
  (n : â„•) â†’ is-injective is-set-â„• is-set-â„• (add-â„• n)
is-injective-add-â„• zero-â„• k l p = p
is-injective-add-â„• (succ-â„• n) k l p =
  is-injective-add-â„• n k l (is-injective-succ-â„• (add-â„• n k) (add-â„• n l) p)

is-injective-add-â„•' :
  (n : â„•) â†’ is-injective is-set-â„• is-set-â„• (Î» m â†’ add-â„• m n)
is-injective-add-â„•' n k l p =
  is-injective-add-â„• n k l
    (((commutative-add-â„• n k) âˆ™ p) âˆ™ (commutative-add-â„• l n))

is-injective-mul-â„• :
  (n : â„•) â†’ (le-â„• zero-â„• n) â†’ is-injective is-set-â„• is-set-â„• (mul-â„• n)
is-injective-mul-â„• (succ-â„• n) star zero-â„• zero-â„• p = refl
is-injective-mul-â„• (succ-â„• n) star zero-â„• (succ-â„• l) p =
  ind-empty
    ( Eq-â„•-eq
      ( zero-â„•)
      ( succ-â„• (add-â„• (mul-â„• n (succ-â„• l)) l))
      ( ( inv (right-zero-law-mul-â„• n)) âˆ™
        ( ( inv (right-unit-law-add-â„• (mul-â„• n zero-â„•))) âˆ™
          ( p âˆ™ (right-successor-law-add-â„• (mul-â„• n (succ-â„• l)) l)))))
is-injective-mul-â„• (succ-â„• n) star (succ-â„• k) zero-â„• p =
  ind-empty
    ( Eq-â„•-eq
      ( succ-â„• (add-â„• (mul-â„• n (succ-â„• k)) k))
      ( zero-â„•)
      ( ( inv (right-successor-law-add-â„• (mul-â„• n (succ-â„• k)) k)) âˆ™
        ( p âˆ™ ( right-zero-law-mul-â„• (succ-â„• n)))))
is-injective-mul-â„• (succ-â„• n) star (succ-â„• k) (succ-â„• l) p =
  ap succ-â„•
    ( is-injective-mul-â„• (succ-â„• n) star k l
      ( is-injective-add-â„• (succ-â„• n)
        ( mul-â„• (succ-â„• n) k)
        ( mul-â„• (succ-â„• n) l)
        ( ( inv (right-successor-law-mul-â„• (succ-â„• n) k) âˆ™ p) âˆ™
          ( right-successor-law-mul-â„• (succ-â„• n) l))))

is-emb-mul-â„• :
  (n : â„•) â†’ (le-â„• zero-â„• n) â†’ is-emb (mul-â„• n)
is-emb-mul-â„• n le =
  is-emb-is-injective is-set-â„• is-set-â„•
    ( mul-â„• n)
    ( is-injective-mul-â„• n le)

is-emb-mul-â„•' :
  (n : â„•) â†’ (le-â„• zero-â„• n) â†’ is-emb (Î» m â†’ mul-â„• m n)
is-emb-mul-â„•' n t =
  is-emb-htpy'
    ( mul-â„• n)
    ( Î» m â†’ mul-â„• m n)
    ( commutative-mul-â„• n)
    ( is-emb-mul-â„• n t)

{- We conclude that the division relation is a property. -}

is-prop-div-â„• :
  (m n : â„•) â†’ (le-â„• zero-â„• m) â†’ is-prop (div-â„• m n)
is-prop-div-â„• (succ-â„• m) n star =
  is-prop-map-is-emb
    ( Î» z â†’ mul-â„• z (succ-â„• m))
    ( is-emb-mul-â„•' (succ-â„• m) star)
    n

{- Next, we show that the division relation is decidable. We do this by showing
   that for any strictly monotone map f : â„• â†’ â„•, any fiber of f is decidable. -}

is-monotone-endo-â„• :
  (f : â„• â†’ â„•) â†’ UU lzero
is-monotone-endo-â„• f = (m n : â„•) â†’ (leq-â„• m n) â†’ (leq-â„• (f m) (f n))

is-strictly-monotone-endo-â„• :
  (f : â„• â†’ â„•) â†’ UU lzero
is-strictly-monotone-endo-â„• f = (m n : â„•) â†’ (le-â„• m n) â†’ (le-â„• (f m) (f n))

is-decidable-fib-endo-â„• :
  (f : â„• â†’ â„•) â†’ is-strictly-monotone-endo-â„• f â†’ (n : â„•) â†’ decide (fib f n)
is-decidable-fib-endo-â„• f H n = {!!}

is-decidable-div-â„• :
  (m n : â„•) â†’ (le-â„• zero-â„• m) â†’ decide (div-â„• m n)
is-decidable-div-â„• m n t = {!!}

-- Exercises

-- Exercise 10.?

Eq-ğŸš-eq : (x y : bool) â†’ Id x y â†’ Eq-ğŸš x y
Eq-ğŸš-eq x .x refl = reflexive-Eq-ğŸš x

abstract
  has-decidable-equality-ğŸš : has-decidable-equality bool
  has-decidable-equality-ğŸš true true = inl refl
  has-decidable-equality-ğŸš true false = inr (Eq-ğŸš-eq true false)
  has-decidable-equality-ğŸš false true = inr (Eq-ğŸš-eq false true)
  has-decidable-equality-ğŸš false false = inl refl

-- Exercise 10.?

abstract
  has-decidable-equality-prod' : {l1 l2 : Level} {A : UU l1} {B : UU l2} â†’
    (x x' : A) (y y' : B) â†’ decide (Id x x') â†’ decide (Id y y') â†’
    decide (Id (pair x y) (pair x' y'))
  has-decidable-equality-prod' x x' y y' (inl p) (inl q) =
    inl (eq-pair-triv (pair p q))
  has-decidable-equality-prod' x x' y y' (inl p) (inr g) =
    inr (Î» h â†’ g (ap pr2 h))
  has-decidable-equality-prod' x x' y y' (inr f) (inl q) =
    inr (Î» h â†’ f (ap pr1 h))
  has-decidable-equality-prod' x x' y y' (inr f) (inr g) =
    inr (Î» h â†’ f (ap pr1 h))

abstract
  has-decidable-equality-prod : {l1 l2 : Level} {A : UU l1} {B : UU l2} â†’
    has-decidable-equality A â†’ has-decidable-equality B â†’
    has-decidable-equality (A Ã— B)
  has-decidable-equality-prod dec-A dec-B (pair x y) (pair x' y') =
    has-decidable-equality-prod' x x' y y' (dec-A x x') (dec-B y y')

-- Exercise 10.?

decide-retract-of :
  {l1 l2 : Level} {A : UU l1} {B : UU l2} â†’
  A retract-of B â†’ decide B â†’ decide A
decide-retract-of (pair i (pair r H)) (inl b) = inl (r b)
decide-retract-of (pair i (pair r H)) (inr f) = inr (f âˆ˜ i)

abstract
  has-decidable-equality-retract-of :
    {l1 l2 : Level} {A : UU l1} {B : UU l2} â†’
    A retract-of B â†’ has-decidable-equality B â†’ has-decidable-equality A
  has-decidable-equality-retract-of (pair i (pair r H)) d x y =
    decide-retract-of
      ( Id-retract-of-Id (pair i (pair r H)) x y)
      ( d (i x) (i y))


{-

is-bounded-fam-â„• :
  {l : Level} (n : â„•) (P : â„• â†’ UU l) â†’ UU l
is-bounded-fam-â„• n P = (m : â„•) â†’ P m â†’ leq-â„• m n

bounds-fam-â„• :
  {l : Level} (P : â„• â†’ UU l) â†’ UU l
bounds-fam-â„• P = Î£ â„• (Î» n â†’ is-bounded-fam-â„• n P)

is-minimal-â„• :
  {l : Level} (P : â„• â†’ UU l) â†’ Î£ â„• P â†’ UU l
is-minimal-â„• P (pair n p) = (t : Î£ â„• P) â†’ leq-â„• n (pr1 t)

eq-zero-leq-zero-â„• :
  (n : â„•) â†’ leq-â„• n zero-â„• â†’ Id n zero-â„•
eq-zero-leq-zero-â„• zero-â„• star = refl
eq-zero-leq-zero-â„• (succ-â„• n) ()

fam-succ-â„• :
  {l : Level} â†’ (â„• â†’ UU l) â†’ (â„• â†’ UU l)
fam-succ-â„• P n = P (succ-â„• n)

decide-fam-succ-â„• :
  {l : Level} (P : â„• â†’ UU l) â†’
  ((n : â„•) â†’ decide (P n)) â†’ ((n : â„•) â†’ decide (P (succ-â„• n)))
decide-fam-succ-â„• P d n = d (succ-â„• n)

min-is-bounded-not-zero-â„• :
  {l : Level} (P : â„• â†’ UU l) â†’ ((n : â„•) â†’ decide (P n)) â†’
  Î£ â„• (Î» n â†’ is-bounded-fam-â„• n P) â†’
  Â¬ (P zero-â„•) â†’
  Î£ (Î£ â„• (fam-succ-â„• P)) (is-minimal-â„• (fam-succ-â„• P)) â†’
  Î£ (Î£ â„• P) (is-minimal-â„• P)
min-is-bounded-not-zero-â„• P d b np0 t = {!!}

min-is-bounded-â„• :
  {l : Level} (P : â„• â†’ UU l) â†’ ((n : â„•) â†’ decide (P n)) â†’
  Î£ â„• (Î» n â†’ is-bounded-fam-â„• n P) â†’
  Î£ â„• P â†’ Î£ (Î£ â„• P) (is-minimal-â„• P)
min-is-bounded-â„• P d (pair zero-â„• b) t =
  pair
    ( pair
      ( zero-â„•)
      ( tr P (eq-zero-leq-zero-â„• (pr1 t) (b (pr1 t) (pr2 t))) (pr2 t)))
    ( Î» p â†’ leq-zero-â„• (pr1 p))
min-is-bounded-â„• P d (pair (succ-â„• n) b) t =
  ind-coprod
    ( Î» (t : decide (P zero-â„•)) â†’ Î£ (Î£ â„• P) (is-minimal-â„• P))
    ( Î» p0 â†’ pair (pair zero-â„• p0) (Î» p â†’ leq-zero-â„• (pr1 p)))
    ( Î» y â†’ min-is-bounded-not-zero-â„• P d (pair (succ-â„• n) b) y
      ( min-is-bounded-â„•
        ( fam-succ-â„• P)
        ( decide-fam-succ-â„• P d)
        {!!}
        {!!}))
    ( d zero-â„•)

{- We show that every non-empty decidable subset of â„• has a least element. -}

least-â„• :
  {l : Level} (P : â„• â†’ UU l) â†’ Î£ â„• P â†’ UU l
least-â„• P (pair n p) = (m : â„•) â†’ P m â†’ leq-â„• n m

least-element-non-empty-decidable-subset-â„• :
  {l : Level} (P : â„• â†’ UU l) (d : (n : â„•) â†’ decide (P n)) â†’
  Î£ â„• P â†’ Î£ (Î£ â„• P) (least-â„• P)
least-element-non-empty-decidable-subset-â„• P d (pair zero-â„• p) =
  pair (pair zero-â„• p) {!!}
least-element-non-empty-decidable-subset-â„• P d (pair (succ-â„• n) p) = {!!}
-}

zero-Fin :
  (n : â„•) â†’ Fin (succ-â„• n)
zero-Fin zero-â„• = inr star
zero-Fin (succ-â„• n) = inl (zero-Fin n)

succ-Fin :
  (n : â„•) â†’ Fin n â†’ Fin n
succ-Fin (succ-â„• n) (inr star) = zero-Fin n
succ-Fin (succ-â„• (succ-â„• n)) (inl (inl x)) = inl (succ-Fin (succ-â„• n) (inl x))
succ-Fin (succ-â„• (succ-â„• n)) (inl (inr star)) = inr star

iterated-succ-Fin :
  (k : â„•) â†’ (n : â„•) â†’ Fin n â†’ Fin n
iterated-succ-Fin zero-â„• n = id
iterated-succ-Fin (succ-â„• k) n = (succ-Fin n) âˆ˜ (iterated-succ-Fin k n)

quotient-â„•-Fin :
  (n : â„•) â†’ Fin (succ-â„• n)
quotient-â„•-Fin n = iterated-succ-Fin n (succ-â„• n) (zero-Fin n)

pred-Fin :
  (n : â„•) â†’ Fin n â†’ Fin n
pred-Fin (succ-â„• zero-â„•) (inr star) = inr star
pred-Fin (succ-â„• (succ-â„• n)) (inl x) = {!!}
pred-Fin (succ-â„• (succ-â„• n)) (inr star) = inl (inr star)

add-Fin :
  (n : â„•) â†’ Fin n â†’ Fin n â†’ Fin n
add-Fin (succ-â„• n) (inl x) j = {!!}
add-Fin (succ-â„• n) (inr x) j = {!!}


idempotent-succ-Fin :
  (n : â„•) (i : Fin n) â†’ Id (iterated-succ-Fin n n i) i
idempotent-succ-Fin (succ-â„• zero-â„•) (inr star) = refl
idempotent-succ-Fin (succ-â„• (succ-â„• n)) (inl x) = {!!}
idempotent-succ-Fin (succ-â„• (succ-â„• n)) (inr x) = {!!}

in-nat-â„¤ : â„• â†’ â„¤
in-nat-â„¤ zero-â„• = zero-â„¤
in-nat-â„¤ (succ-â„• n) = in-pos n

div-â„¤ :
  (k l : â„¤) â†’ UU lzero
div-â„¤ k l = Î£ â„¤ (Î» x â†’ Id (mul-â„¤ x k) l)

_â‰¡_mod_ :
  (k l : â„¤) (n : â„•) â†’ UU lzero
k â‰¡ l mod n = div-â„¤ (in-nat-â„¤ n) (add-â„¤ k (neg-â„¤ l))
